LinkedBetree state machine roughed out

Splinter/Betree/LinkedBetree.i.dfy
@@ -4,45 +4,591 @@
 include "PivotBetree.i.dfy"
 include "../../lib/Buckets/BoundedPivotsLib.i.dfy"
 include "../Journal/GenericDisk.i.dfy"
-
+include "Domain.i.dfy"
 
 module LinkedBetree
 {
-  import opened Options
-  import opened KeyType
-  import opened ValueMessage
-  import opened MsgHistoryMod
-  import opened LSNMod
-  import opened Buffers
-  import GenericDisk
   import opened BoundedPivotsLib
+  import opened Buffers
+  import opened DomainMod
+  import opened GenericDisk
+  import opened KeyType
+//  import opened Lexicographic_Byte_Order
+  import opened LSNMod
+  import opened MemtableMod
+  import opened MsgHistoryMod
+  import opened Options
+  import opened Sequences
+  import opened StampedMod
+  import opened Upperbounded_Lexicographic_Byte_Order_Impl
+  import opened Upperbounded_Lexicographic_Byte_Order_Impl.Ord
+  import opened ValueMessage
+  import opened Maps
+  import TotalKMMapMod
 
   type Pointer = GenericDisk.Pointer
   type Address = GenericDisk.Address
+  type StampedBetree = Stamped<LinkedBetree>
+
+  type Element = Upperbounded_Lexicographic_Byte_Order_Impl.Ord.Element
 
   datatype TransitionLabel =
       QueryLabel(endLsn: LSN, key: Key, value: Value)
     | PutLabel(puts: MsgHistory)
     | QueryEndLsnLabel(endLsn: LSN)
-    | FreezeAsLabel(linkedBetree: LinkedBetree)
+    | FreezeAsLabel(linkedBetree: StampedBetree)
     | InternalLabel()
 
 
-  datatype BetreeNode = Nil | BetreeNode(
+  datatype BetreeNode = BetreeNode(
     buffers: BufferStack,  // Should buffer stack also be linked via pointers?
     pivotTable: PivotTable,
     children: seq<Pointer>)
-  {}
+  {
+    predicate WF() {
+      && (BetreeNode? ==>
+          && WFPivots(pivotTable)
+          && |children| == NumBuckets(pivotTable)
+        )
+    }
 
+    predicate ValidChildIndex(childIdx: nat)
+    {
+      && BetreeNode?
+      && childIdx < NumBuckets(pivotTable)
+    }
+
+    function PushBufferStack(bufferStack: BufferStack) : (out: BetreeNode)
+      requires WF()
+      requires BetreeNode?
+      ensures out.WF()
+    {
+      BetreeNode(buffers.PushBufferStack(bufferStack), pivotTable, children)
+    }
+
+    function ApplyFilter(filter: Domain) : (out: BetreeNode)
+      requires WF()
+      ensures out.WF()
+    {
+      BetreeNode(buffers.ApplyFilter(filter.KeySet()), pivotTable, children)
+    }
+
+    function ChildDomain(childIdx: nat) : (out: Domain)
+      requires WF()
+      requires BetreeNode?
+      requires ValidChildIndex(childIdx)
+      ensures out.WF()
+    {
+      var out := Domain(pivotTable[childIdx], pivotTable[childIdx+1]);
+      reveal_IsStrictlySorted();  /* jonh suspicious lt leak */
+      out.reveal_SaneKeys();  /* jonh suspicious lt leak */
+      out
+    }
+
+    predicate KeyInDomain(key: Key)
+    {
+      && WF()
+      && BetreeNode?
+      && BoundedKey(pivotTable, key)
+    }
+
+    // Redundant; should equal domain.KeySet() for the domain specified by the pivotTable.
+    function KeySet() : iset<Key>
+      requires WF()
+      requires BetreeNode?  // TODO(jonh): trouble for Nils?
+    {
+      iset key | KeyInDomain(key)
+    }
+
+    function ChildPtr(key: Key) : Pointer
+      requires WF()
+      requires BetreeNode?
+      requires KeyInDomain(key)
+    {
+      children[Route(pivotTable, key)]
+    }
+  }
+
+  function TotalPivotTable() : PivotTable
+  {
+    [TotalDomain().start, TotalDomain().end]
+  }
+
+  function EmptyRoot(domain: Domain) : (out: BetreeNode)
+    requires domain.WF()
+    requires domain.Domain?
+    ensures out.WF()
+  {
+    var pivotTable := [domain.start, domain.end];
+    domain.reveal_SaneKeys();  /* jonh suspicious lt leak */
+    assert Keyspace.IsStrictlySorted(pivotTable) by { reveal_IsStrictlySorted(); }  /* jonh suspicious lt leak */
+    BetreeNode(BufferStack([]), pivotTable, [None])
+  }
 
   datatype DiskView = DiskView(seqEnd: LSN, entries: map<Address, BetreeNode>) 
-  {}
+  {
+    // TODO(jonh): some duplication with LinkedJournal.DiskView; refactor into library superclassish thing?
+    // Or a generic with GenericDisk.DiskView<T>?
+    predicate EntriesWF()
+    {
+      (forall addr | addr in entries :: entries[addr].WF())
+    }
+
+    predicate IsNondanglingPointer(ptr: Pointer)
+    {
+      ptr.Some? ==> ptr.value in entries
+    }
+
+    predicate NodeHasNondanglingPointers(node: BetreeNode)
+    {
+      node.BetreeNode? ==>
+      (forall idx:nat | idx < |node.children| :: IsNondanglingPointer(node.children[idx]))
+    }
+
+    predicate NondanglingPointers()
+    {
+      (forall addr | addr in entries :: NodeHasNondanglingPointers(entries[addr]))
+    }
+
+    predicate WF()
+    {
+      && EntriesWF()
+      && NondanglingPointers()
+    }   
+
+    function Get(ptr: Pointer) : BetreeNode
+      requires WF()
+      requires IsNondanglingPointer(ptr)
+      requires ptr.Some?
+    {
+      entries[ptr.value]
+    }
+
+    predicate AgreesWithDisk(other: DiskView)
+    {
+      MapsAgree(entries, other.entries)
+    }
+  }
   
-  
+  // This is the unit of interpretation: A LinkedBetree has enough info in it to interpret to a PivotBetree.BetreeNode.
   datatype LinkedBetree = LinkedBetree(
     root: Pointer,
     diskView: DiskView
-  ) {}
+  )
+  {
+    predicate WF() {
+      && diskView.WF()
+      && diskView.IsNondanglingPointer(root)
+    }
 
+    predicate HasRoot() {
+      && WF()
+      && root.Some?
+    }
 
+    function Root() : BetreeNode
+      requires HasRoot()
+    {
+      diskView.Get(root)
+    }
+
+    function Child(key: Key) : LinkedBetree
+      requires HasRoot()
+      requires Root().KeyInDomain(key)
+    {
+      LinkedBetree(Root().ChildPtr(key), diskView)
+    }
+  }
+
+  datatype Variables = Variables(
+    memtable: Memtable,
+    linked: LinkedBetree)
+  {
+    predicate WF() {
+      && linked.WF()
+    }
+  }
+
+  // TODO(jonh): SO much copypasta from PivotBetree! Library, paramaterize child mechanism?
+  datatype QueryReceiptLine = QueryReceiptLine(
+    ptr: Pointer,
+    result: Message)
+  {
+    predicate WF()
+    {
+      && result.Define?
+    }
+  }
+
+  datatype QueryReceipt = QueryReceipt(
+    key: Key,
+    diskView: DiskView,
+    lines: seq<QueryReceiptLine>)
+  {
+    predicate Structure()
+    {
+      && 0 < |lines|
+      && (forall i:nat | i < |lines| :: lines[i].ptr.Some? <==> i < |lines|-1)
+      && (forall i:nat | i < |lines|-1 :: diskView.IsNondanglingPointer(lines[i].ptr))
+      && Last(lines).result == Define(DefaultValue())
+      && diskView.WF()
+    }
+
+    function Node(i: nat) : (out:BetreeNode)
+      requires Structure()
+      requires i < |lines| - 1  // last line is None ptr
+      ensures out.WF()
+    {
+      diskView.Get(lines[i].ptr)
+    }
+
+    predicate AllLinesWF()
+    {
+      && Structure()
+      && (forall i:nat | i < |lines|-1 :: Node(i).KeyInDomain(key))
+    }
+
+    predicate ChildLinkedAt(i: nat)
+      requires AllLinesWF()
+      requires i < |lines|-1
+    {
+      lines[i+1].ptr == Node(i).ChildPtr(key)
+    }
+
+    function ResultAt(i: nat) : Message
+      requires i < |lines|
+    {
+      lines[i].result
+    }
+
+    predicate ResultLinkedAt(i: nat)
+      requires Structure()
+      requires AllLinesWF()
+      requires i < |lines| - 1
+    {
+      && lines[i].result == Merge(Node(i).buffers.Query(key), ResultAt(i+1))
+    }
+
+    predicate Valid()
+    {
+      && Structure()
+      && AllLinesWF()
+      && (forall i:nat | i < |lines| - 1 :: ChildLinkedAt(i))
+      && (forall i:nat | i < |lines| - 1 :: ResultLinkedAt(i))
+    }
+
+    predicate ValidFor(linked: LinkedBetree, key: Key)
+    {
+      && Valid()
+      && this.diskView == linked.diskView
+      && this.lines[0].ptr == linked.root
+      && this.key == key
+    }
+
+    function Result() : Message
+      requires Structure()
+    {
+      ResultAt(0)
+    }
+  }
+
+  predicate Query(v: Variables, v': Variables, lbl: TransitionLabel, receipt: QueryReceipt)
+  {
+    && lbl.QueryLabel?
+    && lbl.endLsn == v.memtable.seqEnd
+    && receipt.ValidFor(v.linked, lbl.key)
+    && Define(lbl.value) == Merge(v.memtable.Query(lbl.key), receipt.Result())
+    && v' == v
+  }
+
+  predicate Put(v: Variables, v': Variables, lbl: TransitionLabel)
+  {
+    && lbl.PutLabel?
+    && lbl.puts.WF()
+    && lbl.puts.seqStart == v.memtable.seqEnd
+    && v' == v.(
+        memtable := v.memtable.ApplyPuts(lbl.puts)
+      )
+  }
+
+  predicate QueryEndLsn(v: Variables, v': Variables, lbl: TransitionLabel)
+  {
+    && lbl.QueryEndLsnLabel?
+    && lbl.endLsn == v.memtable.seqEnd
+    && v' == v
+  }
+
+  predicate FreezeAs(v: Variables, v': Variables, lbl: TransitionLabel)
+  {
+    && lbl.FreezeAsLabel?
+    && v.WF()
+    && v.memtable.IsEmpty()
+    && lbl.linkedBetree == Stamped(v.linked, v.memtable.seqEnd)
+    && v' == v
+  }
+
+  predicate InternalFlushMemtable(v: Variables, v': Variables, lbl: TransitionLabel)
+  {
+    && v.WF()
+    && var newBuffer := Buffer(v.memtable.mapp);
+    && v'.linked.diskView.AgreesWithDisk(v.linked.diskView)
+      // NB: linked.WF() ==> No nondangling pointers, so in practice linked <= linked'
+    && v'.linked.HasRoot()
+    && var newBuffers := BufferStack([newBuffer]);
+    && v'.linked.Root() == (
+      if !v.linked.HasRoot()
+      then
+        // Tony: Avoiding Promote(). You're welcome. :v)
+        BetreeNode(newBuffers, TotalPivotTable(), [None])
+      else
+        v.linked.Root().PushBufferStack(newBuffers)
+      )
+  }
+  
+  datatype Path = Path(key: Key, depth: nat)
+  {
+    // Valid is defined with respect to some DiskView; it checks whether the key can be routed to depth.
+    function Subpath() : (out: Path)
+      requires 0 < depth
+    {
+      Path(key, depth-1)
+    }
+
+    predicate Valid(linked: LinkedBetree)
+      decreases depth
+    {
+      && linked.WF()
+      && linked.root.Some?
+      && linked.Root().KeyInDomain(key)
+      && (0 < depth ==> Subpath().Valid(linked.Child(key)))
+    }
+
+    function Target(linked: LinkedBetree) : (out: LinkedBetree)
+      requires Valid(linked)
+      ensures out.WF()
+      ensures out.root.Some?
+      decreases depth
+    {
+      if 0 == depth
+      then linked
+      else Subpath().Target(linked.Child(key))
+    }
+
+    predicate IsSubstitution(linked: LinkedBetree, linked': LinkedBetree)
+      decreases depth
+    {
+      && Valid(linked)
+      && Valid(linked')
+      && linked.diskView.AgreesWithDisk(linked'.diskView)
+      // When depth==0, linked.root==linked'.root, so we're done.
+      && var root := linked.Root();
+      && var root' := linked'.Root();
+      // "local" info matches
+      && root.buffers == root'.buffers
+      && root.pivotTable == root'.pivotTable
+      && |root.children| == |root'.children|
+      && (forall childIdx | 0 <= childIdx < |root.children|
+        // All children are either identical (off the key path) or we aren't at
+        // Target() yet (0<depth) and the child obeys Substitution
+        :: if 0<depth && childIdx == Route(root.pivotTable, key)
+            then Subpath().IsSubstitution(
+              LinkedBetree(root.children[childIdx], linked.diskView),
+              LinkedBetree(root'.children[childIdx], linked'.diskView))
+            else
+              // identical pointers, and hence identical subtrees
+              root.children[childIdx] == root'.children[childIdx]
+      )
+    }
+  }
+
+  predicate InternalGrow(v: Variables, v': Variables, lbl: TransitionLabel, step: Step)
+  {
+    && v.WF()
+    && lbl.InternalLabel?
+    && step.InternalGrowStep?
+    && v.linked.HasRoot()
+
+    && v'.linked.diskView.AgreesWithDisk(v.linked.diskView)
+    && v'.linked.HasRoot()
+    && v'.linked.Root() == BetreeNode(BufferStack([]), TotalPivotTable(), [v.linked.root])
+    && v'.memtable == v.memtable  // UNCHANGED
+  }
+
+  predicate IsSplit(linked: LinkedBetree, linked': LinkedBetree, childIdx: nat, splitKey: Key)
+  {
+    && linked.WF()
+    && linked'.WF()
+    && linked.HasRoot()
+    && linked'.HasRoot()
+    && linked'.diskView.AgreesWithDisk(linked.diskView)
+    && var root := linked.Root();
+    && var root' := linked'.Root();
+
+    && root.ValidChildIndex(childIdx)
+    && PivotInsertable(root.pivotTable, childIdx, splitKey)
+    && 0 < childIdx < NumBuckets(root.pivotTable) // Split can't extend domain of this node.
+    && var oldChildPtr := root.children[childIdx];
+    && oldChildPtr.Some?
+
+    // Parent adds splitKey pivot; replaces child at childIdx with two children
+    && root'.ValidChildIndex(childIdx+1)  // obvious once we have replace1with2, but we're not there yet
+    && var leftChildPtr := root'.children[childIdx];
+    && var rightChildPtr := root'.children[childIdx+1];
+    && root' == root.(
+      pivotTable := InsertPivot(root.pivotTable, childIdx, splitKey),
+      children := replace1with2(root.children, leftChildPtr, rightChildPtr, childIdx)
+      )
+
+    // Children get correspending slices
+    && leftChildPtr.Some?
+    && rightChildPtr.Some?
+    && var oldChild := linked.diskView.Get(oldChildPtr);
+    && var leftChild := linked'.diskView.Get(leftChildPtr);
+    && var rightChild := linked'.diskView.Get(rightChildPtr);
+    && leftChild == oldChild.ApplyFilter(Domain(root.pivotTable[childIdx-1], Element(splitKey)))
+    && rightChild == oldChild.ApplyFilter(Domain(Element(splitKey), root.pivotTable[childIdx]))
+
+    // TODO(jonh): Say, ApplyFilter only affects buffers, but we also need to
+    // carve up the pivot tables and children! ...in PivotBetree, too.
+  }
+
+  predicate InternalSplit(v: Variables, v': Variables, lbl: TransitionLabel, step: Step)
+  {
+    && v.WF()
+    && lbl.InternalLabel?
+    && step.InternalSplitStep?
+    && step.path.Valid(v.linked)
+    // v && v' agree on everything down to Target()
+    && step.path.IsSubstitution(v.linked, v'.linked)
+    // Target and Target' are related by a split operation
+    && IsSplit(step.path.Target(v.linked), step.path.Target(v'.linked), step.childIdx, step.splitKey)
+    && v'.memtable == v.memtable  // UNCHANGED
+  }
+
+  // Is linked'.Root() a Flush(childIdx) of linked.Root()?
+  predicate IsFlush(linked: LinkedBetree, linked': LinkedBetree, childIdx: nat)
+  {
+    && linked.WF()
+    && linked'.WF()
+    && linked.HasRoot()
+    && linked'.HasRoot()
+    && linked'.diskView.AgreesWithDisk(linked.diskView)
+    && var root := linked.Root();
+    && var root' := linked'.Root();
+
+    && root.ValidChildIndex(childIdx)
+
+    && var keepKeys := AllKeys() - root.ChildDomain(childIdx).KeySet();
+    && var keptBuffers := root.buffers.ApplyFilter(keepKeys);
+    && var movedBuffers := root.buffers.ApplyFilter(root.ChildDomain(childIdx).KeySet());
+
+    // Parent changes buffers & child at childIdx
+    && root'.buffers == keptBuffers
+    && root'.pivotTable == root.pivotTable
+    && root'.children == root.children[childIdx := root'.children[childIdx]]  // this pointer is allowed to change
+
+    // Flushed childs are nearly identical, except for buffers
+    && root.children[childIdx].Some?
+    && root'.children[childIdx].Some?
+    && var child := linked.diskView.Get(root.children[childIdx]);
+    && var child' := linked'.diskView.Get(root'.children[childIdx]);
+
+    && child'.buffers == child.buffers.PushBufferStack(movedBuffers)
+    && child'.pivotTable == child.pivotTable
+    && child'.children == child.children
+  }
+
+  // The flush step reaches down a path and applies IsFlush.
+  predicate InternalFlush(v: Variables, v': Variables, lbl: TransitionLabel, step: Step)
+  {
+    // An advantage of predicate-style is that we don't have to explicitly
+    // declare BuildTight() (garbage collection); we can leave that to a lower
+    // layer.
+    && v.WF()
+    && lbl.InternalLabel?
+    && step.InternalFlushStep?
+    && step.path.Valid(v.linked)
+    // v && v' agree on everything down to Target()
+    && step.path.IsSubstitution(v.linked, v'.linked)
+    // Target and Target' are related by a flush operation
+    && IsFlush(step.path.Target(v.linked), step.path.Target(v'.linked), step.childIdx)
+    && v'.memtable == v.memtable  // UNCHANGED
+  }
+
+  predicate IsCompaction(linked: LinkedBetree, linked': LinkedBetree)
+  {
+    && linked.WF()
+    && linked'.WF()
+    && linked.HasRoot()
+    && linked'.HasRoot()
+    && linked'.diskView.AgreesWithDisk(linked.diskView) // so that the unchanged children represent the same thing
+
+    && linked'.Root().buffers.Equivalent(linked.Root().buffers)
+    // Can only make a local change; entirety of children subtrees are identical.
+    && linked'.Root().pivotTable == linked.Root().pivotTable  // UNCHANGED
+    && linked'.Root().children == linked.Root().children  // UNCHANGED
+  }
+
+  // NB we tell you exactly how to Split and Flush, but leave lots of
+  // nondetermistic freedom in the description of Compact.
+  predicate InternalCompact(v: Variables, v': Variables, lbl: TransitionLabel, step: Step)
+  {
+    && v.WF()
+    && lbl.InternalLabel?
+    && step.InternalCompactStep?
+    && step.path.Valid(v.linked)
+    // v && v' agree on everything down to Target()
+    && step.path.IsSubstitution(v.linked, v'.linked)
+    // Target and Target' are related by a compaction operation
+    && IsCompaction(step.path.Target(v.linked), step.path.Target(v'.linked))
+    && v'.memtable == v.memtable  // UNCHANGED
+  }
+
+  // public:
+
+  predicate Init(v: Variables, stampedBetree: StampedBetree)
+  {
+    && stampedBetree.value.WF()
+    && v == Variables(EmptyMemtable(stampedBetree.seqEnd), stampedBetree.value)
+  }
+
+  datatype Step =
+      QueryStep(receipt: QueryReceipt)
+    | PutStep()
+    | QueryEndLsnStep()
+    | FreezeAsStep()
+    | InternalGrowStep()
+    | InternalSplitStep(path: Path, childIdx: nat, splitKey: Key)
+    | InternalFlushStep(path: Path, childIdx: nat)
+    | InternalCompactStep(path: Path, compactedNode: BetreeNode)
+  {
+    predicate WF() {
+      match this {
+        case QueryStep(receipt) => receipt.Valid()
+        case InternalSplitStep(path, childIdx, splitKey) => true
+        case InternalFlushStep(path, childIdx) => true
+        case InternalCompactStep(path, compactedNode) =>
+          && compactedNode.WF()
+        case _ => true
+      }
+    }
+  }
+
+  predicate NextStep(v: Variables, v': Variables, lbl: TransitionLabel, step: Step)
+  {
+    match step {
+      case QueryStep(receipt) => Query(v, v', lbl, receipt)
+      case PutStep() => Put(v, v', lbl)
+      case QueryEndLsnStep() => QueryEndLsn(v, v', lbl)
+      case FreezeAsStep() => FreezeAs(v, v', lbl)
+      case InternalGrowStep() => InternalGrow(v, v', lbl, step)
+      case InternalSplitStep(_, _, _) => InternalSplit(v, v', lbl, step)
+      case InternalFlushStep(_, _) => InternalFlush(v, v', lbl, step)
+      case InternalCompactStep(_, _) => InternalCompact(v, v', lbl, step)
+    }
+  }
+
+  predicate Next(v: Variables, v': Variables, lbl: TransitionLabel) {
+    exists step: Step :: NextStep(v, v', lbl, step)
+  }
 }
